% Created 2016-11-16 Mi 21:46
\documentclass[11pt]{article}
\usepackage[utf8]{inputenc}
\usepackage[T1]{fontenc}
\usepackage{fixltx2e}
\usepackage{graphicx}
\usepackage{grffile}
\usepackage{longtable}
\usepackage{wrapfig}
\usepackage{rotating}
\usepackage[normalem]{ulem}
\usepackage{amsmath}
\usepackage{textcomp}
\usepackage{amssymb}
\usepackage{capt-of}
\usepackage{hyperref}
\usepackage[english]{babel}
\date{\today}
\title{}
\hypersetup{
 pdfauthor={Aaron},
 pdftitle={},
 pdfkeywords={},
 pdfsubject={},
 pdfcreator={Emacs 25.1.50.2 (Org mode 8.3.6)}, 
 pdflang={English}}
\begin{document}

a)
A = (not (a and b) and (a or b )) or ((a and b) or not (a or b))


\begin{center}
\begin{tabular}{llllllllll}
a & b & not a & not b & a and b & a or b & not (a and b) & not (a or b) & (not a) and (not b) & A\\
\hline
True & True & False & False & True & True & True & False & False & True\\
True & False & False & True & False & True & False & False & False & True\\
False & True & True & False & False & True & True & False & False & True\\
False & False & True & True & False & False & False & True & True & True\\
 &  &  &  &  &  &  &  &  & \\
\end{tabular}
\end{center}

b)
\begin{align*}
  (\neg(a\land b) \land (a \lor b)) \lor ((a\land b) \lor \neg (a \lor b)) \Leftrightarrow&\\ 
  ((\neg a \lor \neg b) \land (a \lor b)) \lor ((a \land b) \lor (\neg a \land \neg b)) \Leftrightarrow&\\
(((\neg a \lor \neg b)\land a) \lor ((\neg a \lor \neg b)\land b)) \lor ((a \land b ) \lor (\neg a \land \neg b)) \Leftrightarrow&\\
  ((\neg a \land a )\lor (a \land \neg b) \lor (\neg a \land b) \lor (\neg b \land b)) \lor (\neg(\neg(a\land b)) \lor (\neg a \land \neg b)) \Leftrightarrow&\\
 (0 \lor (a \land \neg b ) \lor (\neg a \land b) \lor 0) \lor \neg((\neg a \lor \neg b) \land (a \lor b)) \Leftrightarrow&\\
 (0 \lor (a \land \neg b ) \lor (\neg a \land b) \lor 0) \lor (1 \land \neg(\neg a \land b) \land \neg(\neg b \land a) \land 1)\Leftrightarrow&\\
 (0 \lor (a \land \neg b ) \lor (\neg a \land b) \lor 0) \lor (1 \land ( a \lor \neg b) \land (b \lor \neg a) \land 1)\Leftrightarrow& \\
 \neg(1 \land \neg (a \land \neg b) \land \neg(\neg a \land b) \land 1) \lor  (1 \land ( a \lor \neg b) \land (b \lor \neg a) \land 1) \Leftrightarrow&\\
 \neg(1 \land (\neg a \lor b) \land (a \lor \neg b) \land 1) \lor (1 \land (a \land \neg b) \land (b \lor \neg a) \land 1) \Leftrightarrow&\\
 \neg(1 \land (\neg a \lor b) \land (a \lor \neg b) \land 1) \lor (1 \land (\neg a \lor b) \land ( a \lor \neg b )\land 1)\\
\end{align*}
Der letzte Term ist äquivalent zu \(\neg \phi \lor \phi, \phi \in {0,1}\), was immer wahr (1) sein müsste.
\end{document}